specs/lemmas/Spec.SHA2.Lemmas.fst
@@ -29,7 +29,7 @@ let rec ws_aux (a:sha2_alg) (b:block_w a) (t:counter{t < size_k_w a}): Tot (word
 let ws = ws_aux
 
 (* Core shuffling function *)
-let shuffle_core_ (a:sha2_alg) (block:block_w a) (hash:words_state a) (t:counter{t < size_k_w a}): Tot (words_state a) =
+let shuffle_core_ (a:sha2_alg) (block:block_w a) (hash:words_state' a) (t:counter{t < size_k_w a}): Tot (words_state' a) =
   (**) assert(7 <= S.length hash);
   let a0 = hash.[0] in
   let b0 = hash.[1] in
@@ -53,12 +53,12 @@ let shuffle_core_ (a:sha2_alg) (block:block_w a) (hash:words_state a) (t:counter
 let shuffle_core = shuffle_core_
 
 (* Full shuffling function *)
-let shuffle_aux (a:sha2_alg) (hash:words_state a) (block:block_w a): Tot (words_state a) =
+let shuffle_aux (a:sha2_alg) (hash:words_state' a) (block:block_w a): Tot (words_state' a) =
   Spec.Loops.repeat_range 0 (size_k_w a) (shuffle_core a block) hash
 
 #push-options "--max_fuel 1 --max_ifuel 0"
 
-val shuffle_is_shuffle_pre: a:sha2_alg -> hash:words_state a -> block:block_w a ->
+val shuffle_is_shuffle_pre: a:sha2_alg -> hash:words_state' a -> block:block_w a ->
   Lemma (shuffle a hash block == shuffle_aux a hash block)
 let shuffle_is_shuffle_pre a hash block =
   let rec repeati_is_repeat_range #a (n:nat)
@@ -120,13 +120,15 @@ let shuffle_is_shuffle_pre a hash block =
 
 (* Compression function *)
 let update_aux (a:sha2_alg) (hash:words_state a) (block:bytes{S.length block = block_length a}): Tot (words_state a) =
+  let hash, _ = hash in
   let block_w = words_of_bytes a #block_word_length block in
   let hash_1 = shuffle_aux a hash block_w in
-  Lib.Sequence.map2 ( +. ) (hash <: Lib.Sequence.lseq (word a) (state_word_length a)) hash_1
+  Lib.Sequence.map2 ( +. ) (hash <: Lib.Sequence.lseq (word a) (state_word_length a)) hash_1, ()
 
 val update_is_update_pre: a:sha2_alg -> hash:words_state a -> block:bytes{S.length block = block_length a} ->
   Lemma (update a hash block == update_aux a hash block)
 let update_is_update_pre a hash block =
+  let hash, _ = hash in
   let block_w = words_of_bytes a #block_word_length block in
   let hash_1 = shuffle a hash block_w in
   shuffle_is_shuffle_pre a hash block_w;
@@ -142,8 +144,9 @@ let update_is_update_pre a hash block =
   in Classical.forall_intro aux;
   assert (s1 `Seq.equal` s2)
 
-#push-options "--max_fuel 1 --max_ifuel 0 --z3rlimit 200"
+#push-options "--max_fuel 1 --max_ifuel 1 --z3rlimit 200"
 let update_224_256 hash block =
+  assert_norm (words_state SHA2_224 == words_state SHA2_256);
   let rec ws_224_256 (b: block_w SHA2_256) (t:counter{t < size_k_w SHA2_256}):
     Lemma
       (ensures (ws SHA2_224 b t == ws SHA2_256 b t))
@@ -164,7 +167,7 @@ let update_224_256 hash block =
       ws_224_256 b (t - 2)
     end
   in
-  let shuffle_core_224_256 (block:block_w SHA2_256) (hash:words_state SHA2_256) (t:counter{t < size_k_w SHA2_256}):
+  let shuffle_core_224_256 (block:block_w SHA2_256) (hash:words_state' SHA2_256) (t:counter{t < size_k_w SHA2_256}):
     Lemma (ensures (shuffle_core SHA2_224 block hash t == shuffle_core SHA2_256 block hash t))
     [ SMTPat (shuffle_core SHA2_256 block hash t) ]
   =
@@ -182,7 +185,7 @@ let update_224_256 hash block =
     else
       repeat_range_f (min + 1) max f g (f x min)
   in
-  let shuffle_224_256 (hash:words_state SHA2_256) (block:block_w SHA2_256):
+  let shuffle_224_256 (hash:words_state' SHA2_256) (block:block_w SHA2_256):
     Lemma (ensures (shuffle SHA2_224 hash block == shuffle SHA2_256 hash block))
     [ SMTPat (shuffle SHA2_256 hash block) ]
   =
@@ -210,10 +213,11 @@ let update_224_256 hash block =
   reveal_opaque (`%shuffle) shuffle;
   reveal_opaque (`%update) update
 
-
 #pop-options
 
+
 let rec update_multi_224_256 hash blocks =
+  assert_norm (words_state SHA2_224 == words_state SHA2_256);
   if S.length blocks = 0 then
     ()
   else
